Make weak trace theory a little nicer

Weak_Traces.thy
@@ -1,20 +1,19 @@
-section \<open>Weak Traces \label{appndx:weakTraces}\<close>
+section \<open>Weak Traces\<close>
+
 theory Weak_Traces
   imports Main HML_SRBB Expressiveness_Price
 begin
 
-text \<open>The inductive @{term \<open>is_trace_formula\<close>} represents the modal-logical characterization of weak traces HML$_{WT}$.
-In particular:
-\begin{itemize}
-  \item $\top \in$ HML$_{WT}$ encoded by  @{term \<open>is_trace_formula\<close>} \<open>TT\<close>, @{term \<open>is_trace_formula\<close>} @{term \<open>(ImmConj I \<psi>s)\<close>} if \<open>I = {}\<close> and @{term \<open>is_trace_formula\<close>} @{term \<open>(Conj I \<psi>s)\<close>} if \<open>I = {}.\<close>.
-  \item \<open>\<langle>\<epsilon>\<rangle>\<chi>\<close> $\in$ HML$_{WT}$ if \<open>\<phi>\<close> $\in$ HML$_{WT}$ encoded by @{term \<open>is_trace_formula\<close>} @{term \<open>(Internal \<chi>)\<close>} if @{term \<open>is_trace_formula\<close>} \<open>\<chi>\<close>.
-  \item \<open>(\<alpha>)\<phi>\<close> $\in$ HML$_{WT}$ if \<open>\<phi>\<close> $\in$ HML$_{WT}$ encoded by @{term \<open>is_trace_formula\<close>} @{term \<open>(Obs \<alpha> \<phi>)\<close>} if @{term \<open>is_trace_formula\<close>} \<open>\<phi>\<close>.
-  \item \<open>\<And>{(\<alpha>)\<phi>} \<union> \<Psi>\<close> $\in$ HML$_{WT}$ if \<open>\<phi>\<close> $\in$ HML$_{WT}$ and \<open>\<Psi> = {}\<close> encoded by @{term \<open>is_trace_formula\<close>} @{term \<open>(BranchConj \<alpha> \<phi> I \<psi>s)\<close>} if @{term \<open>is_trace_formula\<close>} \<open>\<phi>\<close> and \<open>I = {}\<close>.
-\end{itemize}\<close>
+text \<open>
+  The point of this theory is to prove that the coordinate \<^term>\<open>(E \<infinity> 0 0 0 0 0 0 0)\<close> precisely characterizes weak trace preorder and equivalence.
+\<close>
+
+subsection \<open>Weak Traces as Modal Constructs\<close>
 
 inductive
-      is_trace_formula :: \<open>('act, 'i) hml_srbb \<Rightarrow> bool\<close>
-  and is_trace_formula_inner :: \<open>('act, 'i) hml_srbb_inner \<Rightarrow> bool\<close> where
+  is_trace_formula :: \<open>('act, 'i) hml_srbb \<Rightarrow> bool\<close> and
+  is_trace_formula_inner :: \<open>('act, 'i) hml_srbb_inner \<Rightarrow> bool\<close>
+where
   \<open>is_trace_formula TT\<close> |
   \<open>is_trace_formula (Internal \<chi>)\<close> if \<open>is_trace_formula_inner \<chi>\<close> |
   \<open>is_trace_formula (ImmConj I \<psi>s)\<close> if \<open>I = {}\<close> |
@@ -23,9 +22,11 @@ inductive
   \<open>is_trace_formula_inner (Conj I \<psi>s)\<close> if \<open>I = {}\<close>
 
 text \<open>We define a function that translates a (weak) trace \<open>tr\<close> to a formula \<open>\<phi>\<close> such that a state \<open>p\<close> models \<open>\<phi>\<close>, \<open>p \<Turnstile> \<phi>\<close> if and only if \<open>tr\<close> is a (weak) trace of \<open>p\<close>.\<close>
-fun wtrace_to_srbb :: \<open>'act list \<Rightarrow> ('act, 'i) hml_srbb\<close>
-  and wtrace_to_inner :: \<open>'act list \<Rightarrow> ('act, 'i) hml_srbb_inner\<close>
-  and wtrace_to_conjunct :: \<open>'act list \<Rightarrow> ('act, 'i) hml_srbb_conjunct\<close> where
+fun
+  wtrace_to_srbb :: \<open>'act list \<Rightarrow> ('act, 'i) hml_srbb\<close> and
+  wtrace_to_inner :: \<open>'act list \<Rightarrow> ('act, 'i) hml_srbb_inner\<close> and
+  wtrace_to_conjunct :: \<open>'act list \<Rightarrow> ('act, 'i) hml_srbb_conjunct\<close>
+where
   \<open>wtrace_to_srbb [] = TT\<close> |
   \<open>wtrace_to_srbb tr = (Internal (wtrace_to_inner tr))\<close> |
 
@@ -34,24 +35,28 @@ fun wtrace_to_srbb :: \<open>'act list \<Rightarrow> ('act, 'i) hml_srbb\<close>
 
   \<open>wtrace_to_conjunct tr = Pos (wtrace_to_inner tr)\<close> \<comment> \<open>Should never happen\<close>
 
-text \<open>@{term \<open>wtrace_to_srbb trace\<close>} is in our modal-logical characterization of weak traces.\<close>
 lemma trace_to_srbb_is_trace_formula:
   \<open>is_trace_formula (wtrace_to_srbb trace)\<close>
   by (induct trace,
       auto simp add: is_trace_formula.simps is_trace_formula_is_trace_formula_inner.intros(1,4))
 
-text \<open>The following three lemmas show that the modal-logical characterization of HML$_{WT}$ corresponds to the sublanguage of HML$_\text{SRBB}$, obtain by the energy coordinates \<open>(\<infinity>, 0, 0, 0, 0, 0, 0, 0)\<close>.\<close>
+subsection \<open>Weak Trace Observations through Coordinates\<close>
+
+text \<open>The following three lemmas show that the modal-logical characterization of weak traces corresponds to the sublanguage of HML$_\text{SRBB}$, obtain by the energy coordinates \<open>(\<infinity>, 0, 0, 0, 0, 0, 0, 0)\<close>.\<close>
 
 lemma trace_formula_to_expressiveness:
-  fixes \<phi> :: \<open>('act, 'i) hml_srbb\<close>
-  fixes \<chi> :: \<open>('act, 'i) hml_srbb_inner\<close>
+  fixes
+    \<phi> :: \<open>('act, 'i) hml_srbb\<close> and
+    \<chi> :: \<open>('act, 'i) hml_srbb_inner\<close>
   shows  \<open>(is_trace_formula \<phi>       \<longrightarrow> (\<phi> \<in> \<O>       (E \<infinity> 0 0 0 0 0 0 0)))
         \<and> (is_trace_formula_inner \<chi> \<longrightarrow> (\<chi> \<in> \<O>_inner (E \<infinity> 0 0 0 0 0 0 0)))\<close>
-  by (rule is_trace_formula_is_trace_formula_inner.induct) (simp add: Sup_enat_def \<O>_def \<O>_inner_def)+
+  by (rule is_trace_formula_is_trace_formula_inner.induct)
+     (simp add: Sup_enat_def \<O>_def \<O>_inner_def)+
 
 lemma expressiveness_to_trace_formula:
-  fixes \<phi> :: \<open>('act, 'i) hml_srbb\<close>
-  fixes \<chi> :: \<open>('act, 'i) hml_srbb_inner\<close>
+  fixes
+    \<phi> :: \<open>('act, 'i) hml_srbb\<close> and
+    \<chi> :: \<open>('act, 'i) hml_srbb_inner\<close>
   shows \<open>(\<phi> \<in> \<O> (E \<infinity> 0 0 0 0 0 0 0) \<longrightarrow> is_trace_formula \<phi>)
        \<and> (\<chi> \<in> \<O>_inner (E \<infinity> 0 0 0 0 0 0 0) \<longrightarrow> is_trace_formula_inner \<chi>)
        \<and> True\<close>
@@ -78,7 +83,9 @@ next
     assume \<open>Conj I \<psi>s \<in> \<O>_inner (E \<infinity> 0 0 0 0 0 0 0)\<close>
     hence \<open>I = {}\<close>
       unfolding \<O>_inner_def
-      by (metis bot.extremum_uniqueI bot_enat_def energy.sel(3) expr_pr_inner.simps inst_conj_depth_inner.simps(2) le_iff_add leq_components mem_Collect_eq not_one_le_zero)
+      by (metis bot.extremum_uniqueI bot_enat_def energy.sel(3) expr_pr_inner.simps
+          inst_conj_depth_inner.simps(2) le_iff_add leq_components
+          mem_Collect_eq not_one_le_zero)
     then show \<open>is_trace_formula_inner (Conj I \<psi>s)\<close>
       by (simp add: is_trace_formula_is_trace_formula_inner.intros(5))
   qed
@@ -114,43 +121,37 @@ lemma modal_depth_only_is_trace_form:
 context lts_tau
 begin
 
-text \<open>If a formula \<open>\<phi>\<close> is in HML$_{WT}$ and a state \<open>p\<close> models \<open>\<phi>\<close>, then there exists a weak trace \<open>tr\<close> of \<open>p\<close> such that @{term \<open>wtrace_to_srbb tr\<close>} is equivalent to \<open>\<phi>\<close>.\<close>
+text \<open>If a trace formula \<open>\<phi>\<close> is satisfied by a state \<open>p\<close> then there exists a weak trace \<open>tr\<close> of \<open>p\<close> such that @{term \<open>wtrace_to_srbb tr\<close>} is equivalent to \<open>\<phi>\<close>.\<close>
 lemma trace_formula_implies_trace:
-  fixes \<psi> ::\<open>('a, 's) hml_srbb_conjunct\<close>
+  fixes
+    \<psi> ::\<open>('a, 's) hml_srbb_conjunct\<close>
   shows
-       trace_case: \<open>is_trace_formula \<phi> \<Longrightarrow> p \<Turnstile>SRBB \<phi> \<Longrightarrow> (\<exists>tr \<in> weak_traces p. wtrace_to_srbb tr \<Lleftarrow>srbb\<Rrightarrow> \<phi>)\<close>
-    and conj_case: \<open>is_trace_formula_inner \<chi> \<Longrightarrow> hml_srbb_inner_models q \<chi> \<Longrightarrow> (\<exists>tr \<in> weak_traces q. wtrace_to_inner tr \<Lleftarrow>\<chi>\<Rrightarrow> \<chi>)\<close>
-    and            True
+    \<open>is_trace_formula \<phi> \<Longrightarrow> p \<Turnstile>SRBB \<phi>
+      \<Longrightarrow> \<exists>tr \<in> weak_traces p. wtrace_to_srbb tr \<Lleftarrow>srbb\<Rrightarrow> \<phi>\<close>
+    \<open>is_trace_formula_inner \<chi> \<Longrightarrow> hml_srbb_inner_models q \<chi>
+      \<Longrightarrow> \<exists>tr \<in> weak_traces q. wtrace_to_inner tr \<Lleftarrow>\<chi>\<Rrightarrow> \<chi>\<close>
+    True
 proof (induction \<phi> and \<chi> and \<psi> arbitrary: p and q)
   case TT
-  then have \<open>[] \<in> weak_traces p\<close>
+  thus ?case
     using weak_step_sequence.intros(1) silent_reachable.intros(1) by fastforce
-  moreover have \<open>wtrace_to_srbb [] \<Lleftarrow>srbb\<Rrightarrow> TT\<close>
-    unfolding wtrace_to_srbb.simps
-    by (simp add: equivp_reflp)
-  ultimately show ?case by auto
 next
   case (Internal \<chi>)
-
-  from \<open>is_trace_formula (Internal \<chi>)\<close>
-  have \<open>is_trace_formula_inner \<chi>\<close>
-    using is_trace_formula.cases by auto
-
+  hence \<open>is_trace_formula_inner \<chi>\<close>
+    using is_trace_formula.cases by blast
   from \<open>p \<Turnstile>SRBB Internal \<chi>\<close>
-  have \<open>\<exists>p'. p \<Zsurj> p' \<and> hml_srbb_inner_models p' \<chi>\<close>
-    unfolding hml_srbb_models.simps.
-  then obtain p' where \<open>p \<Zsurj> p'\<close> and \<open>hml_srbb_inner_models p' \<chi>\<close> by auto
+    have \<open>\<exists>p'. p \<Zsurj> p' \<and> hml_srbb_inner_models p' \<chi>\<close>
+    unfolding hml_srbb_models.simps .
+  then obtain p' where \<open>p \<Zsurj> p'\<close> \<open>hml_srbb_inner_models p' \<chi>\<close> by auto
   hence \<open>hml_srbb_inner_models p' \<chi>\<close> by auto
   with \<open>is_trace_formula_inner \<chi>\<close>
-  have \<open>\<exists>tr\<in>weak_traces p'. wtrace_to_inner tr \<Lleftarrow>\<chi>\<Rrightarrow> \<chi>\<close>
-    using Internal.IH by blast
+    have \<open>\<exists>tr\<in>weak_traces p'. wtrace_to_inner tr \<Lleftarrow>\<chi>\<Rrightarrow> \<chi>\<close>
+    using Internal by blast
   then obtain tr where tr_spec:
     \<open>tr \<in> weak_traces p'\<close> \<open>wtrace_to_inner tr \<Lleftarrow>\<chi>\<Rrightarrow> \<chi>\<close> by auto
   with \<open>p \<Zsurj> p'\<close> have \<open>tr \<in> weak_traces p\<close>
     using silent_prepend_weak_traces by auto
-
-  moreover
-  have \<open>wtrace_to_srbb tr \<Lleftarrow>srbb\<Rrightarrow> Internal \<chi>\<close>
+  moreover have \<open>wtrace_to_srbb tr \<Lleftarrow>srbb\<Rrightarrow> Internal \<chi>\<close>
   proof (cases tr)
     case Nil
     thus ?thesis
@@ -158,193 +159,93 @@ next
   next
     case (Cons a tr)
     thus ?thesis
-      using tr_spec internal_srbb_cong by auto
+      using tr_spec internal_srbb_cong
+      by (metis wtrace_to_srbb.simps(2))
   qed
-
-  ultimately show ?case by auto
+  ultimately show ?case by blast
 next
   case (ImmConj I \<psi>s)
-
   from \<open>is_trace_formula (ImmConj I \<psi>s)\<close>
   have \<open>I = {}\<close>
     by (simp add: is_trace_formula.simps)
-
   have \<open>[] \<in> weak_traces p\<close>
     using silent_reachable.intros(1) weak_step_sequence.intros(1) by auto
-
-  from srbb_TT_is_empty_conj
-   and \<open>I = {}\<close>
   have \<open>wtrace_to_srbb [] \<Lleftarrow>srbb\<Rrightarrow> ImmConj I \<psi>s\<close>
+    using srbb_TT_is_empty_conj \<open>I = {}\<close>
     unfolding wtrace_to_srbb.simps by auto
-
-  from \<open>[] \<in> weak_traces p\<close>
-   and \<open>wtrace_to_srbb [] \<Lleftarrow>srbb\<Rrightarrow> ImmConj I \<psi>s\<close>
-  show \<open>\<exists>tr\<in>weak_traces p. wtrace_to_srbb tr \<Lleftarrow>srbb\<Rrightarrow> ImmConj I \<psi>s\<close> by auto
+  thus \<open>\<exists>tr\<in>weak_traces p. wtrace_to_srbb tr \<Lleftarrow>srbb\<Rrightarrow> ImmConj I \<psi>s\<close>
+    using \<open>[] \<in> weak_traces p\<close> by auto
 next
   case (Obs \<alpha> \<phi>)
-  assume IH: \<open>\<And>p1. is_trace_formula \<phi> \<Longrightarrow> p1 \<Turnstile>SRBB \<phi> \<Longrightarrow> \<exists>tr\<in>weak_traces p1. wtrace_to_srbb tr \<Lleftarrow>srbb\<Rrightarrow> \<phi>\<close>
-     and \<open>is_trace_formula_inner (Obs \<alpha> \<phi>)\<close>
-     and \<open>hml_srbb_inner_models q (Obs \<alpha> \<phi>)\<close>
-  then show \<open>\<exists>tr \<in> weak_traces q. wtrace_to_inner tr \<Lleftarrow>\<chi>\<Rrightarrow> Obs \<alpha> \<phi>\<close>
+  thus ?case
   proof (cases \<open>\<alpha> = \<tau>\<close>)
     case True
-
     with \<open>hml_srbb_inner_models q (Obs \<alpha> \<phi>)\<close> have \<open>q \<Turnstile>SRBB \<phi>\<close>
       using Obs.prems(1) silent_reachable.step empty_conj_trivial(1)
       by (metis (no_types, lifting) hml_srbb_inner.distinct(1) hml_srbb_inner.inject(1)
           hml_srbb_inner_models.simps(1) hml_srbb_models.simps(1,2) is_trace_formula.cases
           is_trace_formula_inner.cases)
-
     moreover have \<open>is_trace_formula \<phi>\<close>
       using \<open>is_trace_formula_inner (Obs \<alpha> \<phi>)\<close> is_trace_formula_inner.cases by auto
-
     ultimately show \<open>\<exists>tr \<in> weak_traces q. wtrace_to_inner tr \<Lleftarrow>\<chi>\<Rrightarrow> Obs \<alpha> \<phi>\<close>
       using Obs.IH
       by (metis \<open>\<alpha> = \<tau>\<close> obs_srbb_cong prepend_\<tau>_weak_trace wtrace_to_inner.simps(2))
   next
     case False
-
     from \<open>is_trace_formula_inner (Obs \<alpha> \<phi>)\<close>
     have \<open>is_trace_formula \<phi>\<close>
       by (simp add: is_trace_formula_inner.simps)
-
     from \<open>hml_srbb_inner_models q (Obs \<alpha> \<phi>)\<close> and \<open>\<alpha> \<noteq> \<tau>\<close>
     have \<open>\<exists>q'. q \<mapsto> \<alpha> q' \<and> q' \<Turnstile>SRBB \<phi>\<close> by simp
-    then obtain q' where \<open>q \<mapsto> \<alpha> q'\<close> and \<open>q' \<Turnstile>SRBB \<phi>\<close> by auto
-
-    from \<open>is_trace_formula \<phi>\<close>
-     and \<open>q' \<Turnstile>SRBB \<phi>\<close>
-     and IH
-    have \<open>\<exists>tr' \<in> weak_traces q'. wtrace_to_srbb tr' \<Lleftarrow>srbb\<Rrightarrow> \<phi>\<close> by auto
-    then obtain tr' where \<open>tr' \<in> weak_traces q'\<close> and \<open>wtrace_to_srbb tr' \<Lleftarrow>srbb\<Rrightarrow> \<phi>\<close> by auto
-
-    from \<open>q \<mapsto> \<alpha> q'\<close>
-     and \<open>tr' \<in> weak_traces q'\<close>
+    then obtain q' where \<open>q \<mapsto> \<alpha> q'\<close> \<open>q' \<Turnstile>SRBB \<phi>\<close> by auto
+    hence \<open>\<exists>tr' \<in> weak_traces q'. wtrace_to_srbb tr' \<Lleftarrow>srbb\<Rrightarrow> \<phi>\<close>
+      using \<open>is_trace_formula \<phi>\<close> Obs by auto
+    then obtain tr' where \<open>tr' \<in> weak_traces q'\<close> \<open>wtrace_to_srbb tr' \<Lleftarrow>srbb\<Rrightarrow> \<phi>\<close> by auto
     have \<open>(\<alpha> # tr') \<in> weak_traces q\<close>
-      using step_prepend_weak_traces by auto
-
+      using \<open>q \<mapsto> \<alpha> q'\<close> \<open>tr' \<in> weak_traces q'\<close> step_prepend_weak_traces by auto
     from \<open>wtrace_to_srbb tr' \<Lleftarrow>srbb\<Rrightarrow> \<phi>\<close>
     have \<open>Obs \<alpha> (wtrace_to_srbb tr') \<Lleftarrow>\<chi>\<Rrightarrow> Obs \<alpha> \<phi>\<close>
       using obs_srbb_cong by auto
     then have \<open>wtrace_to_inner (\<alpha> # tr') \<Lleftarrow>\<chi>\<Rrightarrow> Obs \<alpha> \<phi>\<close>
       unfolding wtrace_to_inner.simps.
-
     with \<open>(\<alpha> # tr') \<in> weak_traces q\<close>
-    show \<open>\<exists>tr \<in> weak_traces q. wtrace_to_inner tr \<Lleftarrow>\<chi>\<Rrightarrow> Obs \<alpha> \<phi>\<close> by blast
+      show \<open>\<exists>tr \<in> weak_traces q. wtrace_to_inner tr \<Lleftarrow>\<chi>\<Rrightarrow> Obs \<alpha> \<phi>\<close> by blast
   qed
 next
   case (Conj I \<psi>s)
-  assume \<open>is_trace_formula_inner (Conj I \<psi>s)\<close>
-     and \<open>hml_srbb_inner_models q (Conj I \<psi>s)\<close>
-
-  from \<open>is_trace_formula_inner (Conj I \<psi>s)\<close>
-  have \<open>I = {}\<close>
+  from \<open>is_trace_formula_inner (Conj I \<psi>s)\<close> have \<open>I = {}\<close>
     by (simp add: is_trace_formula_inner.simps)
-
-  have \<open>[] \<in> weak_traces q\<close> by (rule empty_trace_allways_weak_trace)
-
   have \<open>(Conj {} (\<lambda>_. undefined)) \<Lleftarrow>\<chi>\<Rrightarrow> (Conj {} \<psi>s)\<close>
     using srbb_obs_\<tau>_is_\<chi>TT by simp
   then have \<open>(Conj {} (\<lambda>_. undefined)) \<Lleftarrow>\<chi>\<Rrightarrow> (Conj I \<psi>s)\<close>
     using \<open>I = {}\<close> by auto
   then have \<open>wtrace_to_inner [] \<Lleftarrow>\<chi>\<Rrightarrow> Conj I \<psi>s\<close>
     unfolding wtrace_to_inner.simps.
+  with empty_trace_allways_weak_trace[of q] show ?case by auto
+qed (auto simp add: is_trace_formula_inner.simps)
 
-  from \<open>[] \<in> weak_traces q\<close>
-   and \<open>wtrace_to_inner [] \<Lleftarrow>\<chi>\<Rrightarrow> Conj I \<psi>s\<close>
-  show ?case by auto
-next
-  case (StableConj I \<psi>s)
-  have \<open>\<not>is_trace_formula_inner (StableConj I \<psi>s)\<close>
-    by (simp add: is_trace_formula_inner.simps)
-  with \<open>is_trace_formula_inner (StableConj I \<psi>s)\<close>
-  show ?case by contradiction
-next
-  case (BranchConj \<alpha> \<phi> I \<psi>s)
-  assume IH: \<open>\<And>p1. is_trace_formula \<phi> \<Longrightarrow> p1 \<Turnstile>SRBB \<phi> \<Longrightarrow> \<exists>tr\<in>weak_traces p1. wtrace_to_srbb tr \<Lleftarrow>srbb\<Rrightarrow> \<phi>\<close>
-  from \<open>is_trace_formula_inner (BranchConj \<alpha> \<phi> I \<psi>s)\<close>
-  have \<open>is_trace_formula \<phi> \<and> I = {}\<close>
-    by (simp add: is_trace_formula_inner.simps)
-  hence \<open>is_trace_formula \<phi>\<close> and \<open>I = {}\<close> by auto
-  from \<open>hml_srbb_inner_models q (BranchConj \<alpha> \<phi> I \<psi>s)\<close>
-   and \<open>I = {}\<close>
-  have \<open>hml_srbb_inner_models q (Obs \<alpha> \<phi>)\<close>
-    using srbb_obs_is_empty_branch_conj
-    by auto
-
-  have \<open>\<exists>tr \<in> weak_traces q. wtrace_to_inner tr \<Lleftarrow>\<chi>\<Rrightarrow> Obs \<alpha> \<phi>\<close>
-  proof (cases \<open>\<alpha> = \<tau>\<close>)
-    assume \<open>\<alpha> = \<tau>\<close>
-
-    from \<open>hml_srbb_inner_models q (Obs \<alpha> \<phi>)\<close>
-    show \<open>\<exists>tr \<in> weak_traces q. wtrace_to_inner tr \<Lleftarrow>\<chi>\<Rrightarrow> Obs \<alpha> \<phi>\<close>
-      using BranchConj.prems(1) is_trace_formula_inner.simps by fastforce
-  next
-    assume \<open>\<alpha> \<noteq> \<tau>\<close>
-
-    from \<open>hml_srbb_inner_models q (Obs \<alpha> \<phi>)\<close>
-     and \<open>\<alpha> \<noteq> \<tau>\<close>
-    have \<open>\<exists>q'. q \<mapsto> \<alpha> q' \<and> q' \<Turnstile>SRBB \<phi>\<close> by auto
-    then obtain q' where \<open>q \<mapsto> \<alpha> q'\<close> and \<open>q' \<Turnstile>SRBB \<phi>\<close> by auto
-
-    from \<open>is_trace_formula \<phi>\<close>
-     and \<open>q' \<Turnstile>SRBB \<phi>\<close>
-     and IH
-    have \<open>\<exists>tr' \<in> weak_traces q'. wtrace_to_srbb tr' \<Lleftarrow>srbb\<Rrightarrow> \<phi>\<close> by auto
-    then obtain tr' where \<open>tr' \<in> weak_traces q'\<close> and \<open>wtrace_to_srbb tr' \<Lleftarrow>srbb\<Rrightarrow> \<phi>\<close> by auto
-
-    from \<open>q \<mapsto> \<alpha> q'\<close>
-     and \<open>tr' \<in> weak_traces q'\<close>
-    have \<open>(\<alpha> # tr') \<in> weak_traces q\<close>
-      using step_prepend_weak_traces by auto
-
-    from \<open>wtrace_to_srbb tr' \<Lleftarrow>srbb\<Rrightarrow> \<phi>\<close>
-    have \<open>Obs \<alpha> (wtrace_to_srbb tr') \<Lleftarrow>\<chi>\<Rrightarrow> Obs \<alpha> \<phi>\<close>
-      using obs_srbb_cong by auto
-    then have \<open>wtrace_to_inner (\<alpha> # tr') \<Lleftarrow>\<chi>\<Rrightarrow> Obs \<alpha> \<phi>\<close>
-      unfolding wtrace_to_inner.simps.
-
-    with \<open>(\<alpha> # tr') \<in> weak_traces q\<close>
-    show \<open>\<exists>tr \<in> weak_traces q. wtrace_to_inner tr \<Lleftarrow>\<chi>\<Rrightarrow> Obs \<alpha> \<phi>\<close> by blast
-  qed
-  then obtain tr where \<open>tr \<in> weak_traces q\<close> and \<open>wtrace_to_inner tr \<Lleftarrow>\<chi>\<Rrightarrow> Obs \<alpha> \<phi>\<close> by auto
-
-  from \<open>wtrace_to_inner tr \<Lleftarrow>\<chi>\<Rrightarrow> Obs \<alpha> \<phi>\<close>
-   and \<open>I = {}\<close>
-  have \<open>wtrace_to_inner tr \<Lleftarrow>\<chi>\<Rrightarrow> (BranchConj \<alpha> \<phi> I \<psi>s)\<close>
-    using srbb_obs_is_empty_branch_conj by simp
-  with \<open>tr \<in> weak_traces q\<close>
-  show ?case by blast
-next
-  case (Pos \<chi>)
-  then show ?case by auto
-next
-  case (Neg \<chi>)
-  then show ?case by auto
-qed
-
-text \<open>\<open>t\<close> is a weak trace of a state \<open>p\<close> if and only if \<open>p\<close> models the formula obtained from @{term \<open>wtrace_to_srbb t\<close>}.\<close>
 lemma trace_equals_trace_to_formula:
-  \<open>t \<in> weak_traces p = (p \<Turnstile>SRBB (wtrace_to_srbb t))\<close>
+  \<open>t \<in> weak_traces p \<longleftrightarrow> p \<Turnstile>SRBB (wtrace_to_srbb t)\<close>
 proof
   assume \<open>t \<in> weak_traces p\<close>
   show \<open>p \<Turnstile>SRBB (wtrace_to_srbb t)\<close>
     using \<open>t \<in> weak_traces p\<close>
-  proof(induction t arbitrary: p)
+  proof (induction t arbitrary: p)
     case Nil
     then show ?case
       by simp
   next
     case (Cons a tail)
-    from Cons obtain p'' p' where \<open>p \<Zsurj>\<mapsto>\<Zsurj> a p''\<close> \<open>p'' \<Zsurj>\<mapsto>\<Zsurj>$ tail p'\<close> using weak_step_sequence.simps
+    then obtain p'' p' where \<open>p \<Zsurj>\<mapsto>\<Zsurj> a p''\<close> \<open>p'' \<Zsurj>\<mapsto>\<Zsurj>$ tail p'\<close>
+      using weak_step_sequence.simps
       by (smt (verit, best) list.discI list.inject mem_Collect_eq)
     with Cons(1) have IS: \<open>p'' \<Turnstile>SRBB wtrace_to_srbb tail\<close>
       by blast
-    from Cons have goal_eq: \<open>wtrace_to_srbb (a # tail) = (Internal (Obs a (wtrace_to_srbb tail)))\<close>
+    from Cons have \<open>wtrace_to_srbb (a # tail) = (Internal (Obs a (wtrace_to_srbb tail)))\<close>
       by simp
-    show ?case
+    thus ?case
       by (smt (verit) Cons.IH IS lts_tau.hml_srbb_inner_models.simps(1)
-          lts_tau.silent_reachable_trans \<open>p \<Zsurj>\<mapsto>\<Zsurj> a p''\<close> empty_trace_allways_weak_trace goal_eq
+          lts_tau.silent_reachable_trans \<open>p \<Zsurj>\<mapsto>\<Zsurj> a p''\<close> empty_trace_allways_weak_trace
           hml_srbb_models.simps(2) weak_step_def wtrace_to_srbb.elims)
   qed
 next
@@ -358,50 +259,28 @@ next
     case (Cons a tail)
     hence \<open>p \<Turnstile>SRBB (Internal (Obs a (wtrace_to_srbb tail)))\<close>
       by simp
-    show ?case
-      using Cons.IH \<open>p \<Turnstile>SRBB hml_srbb.Internal (hml_srbb_inner.Obs a (wtrace_to_srbb tail))\<close> prepend_\<tau>_weak_trace silent_prepend_weak_traces step_prepend_weak_traces by fastforce
+    thus ?case
+      using Cons prepend_\<tau>_weak_trace silent_prepend_weak_traces step_prepend_weak_traces
+      by fastforce
   qed
 qed
 
-text \<open>If a state \<open>p\<close> weakly trace-pre-orders another state \<open>q\<close>, \<open>\<phi>\<close> is in our modal-logical characterization HML$_{WT}$, and \<open>p\<close> models \<open>\<phi>\<close> then \<open>q\<close> models \<open>\<phi>\<close>.\<close>
-lemma aux:
-  fixes \<phi> :: \<open>('a, 's) hml_srbb\<close>
-  fixes \<chi> :: \<open>('a, 's) hml_srbb_inner\<close>
-  fixes \<psi> :: \<open>('a, 's) hml_srbb_conjunct\<close>
-  shows \<open>p \<lesssim>WT q \<Longrightarrow> is_trace_formula \<phi> \<Longrightarrow> p \<Turnstile>SRBB \<phi> \<Longrightarrow> q \<Turnstile>SRBB \<phi>\<close>
-proof -
-  assume \<phi>_trace: \<open>is_trace_formula \<phi>\<close> and p_sat_srbb: \<open>p \<Turnstile>SRBB \<phi>\<close> and assms: \<open>p \<lesssim>WT q\<close>
-  show \<open>q \<Turnstile>SRBB \<phi>\<close>
-  proof -
-    from assms have p_trace_implies_q_trace: \<open>\<forall>tr p'. (p \<Zsurj>\<mapsto>\<Zsurj>$ tr p') \<longrightarrow> (\<exists>q'. q \<Zsurj>\<mapsto>\<Zsurj>$ tr q')\<close>
-      unfolding weakly_trace_preordered_def by auto
-    from p_sat_srbb trace_formula_implies_trace obtain tr p' where
-      \<open>(p \<Zsurj>\<mapsto>\<Zsurj>$ tr p')\<close> \<open>wtrace_to_srbb tr \<Lleftarrow>srbb\<Rrightarrow> \<phi>\<close>
-      using \<phi>_trace by blast
-    with p_trace_implies_q_trace obtain q' where \<open>q \<Zsurj>\<mapsto>\<Zsurj>$ tr q'\<close>
-      by blast
-    with trace_equals_trace_to_formula show ?thesis
-      using \<open>wtrace_to_srbb tr \<Lleftarrow>srbb\<Rrightarrow> \<phi>\<close> by auto
-  qed
-qed
-
-text \<open>These are the main lemmas of this theory. They establish that the colloquial, relational notion of of weak trace pre-order/equivalence
-has the same distinctive power as the one derived from the coordinate (\<open>\<infinity>, 0, 0, 0, 0, 0, 0, 0\<close>).
-\\\\
-A state \<open>p\<close> weakly trace-pre-orders a state \<open>q\<close> iff and only if it also pre-orders \<open>q\<close> with respect to the coordinate (\<open>\<infinity>, 0, 0, 0, 0, 0, 0, 0\<close>).\<close>
 lemma expr_preorder_characterizes_relational_preorder_traces:
   \<open>(p \<lesssim>WT q) = (p \<preceq> (E \<infinity> 0 0 0 0 0 0 0) q)\<close>
   unfolding expr_preord_def preordered_def
 proof
   assume \<open>p \<lesssim>WT q\<close>
   thus \<open>\<forall>\<phi>\<in>\<O> (E \<infinity> 0 0 0 0 0 0 0). p \<Turnstile>SRBB \<phi> \<longrightarrow> q \<Turnstile>SRBB \<phi>\<close>
-    using aux expressiveness_to_trace_formula weakly_trace_preordered_def
-    by blast+
+    using expressiveness_to_trace_formula trace_equals_trace_to_formula
+      trace_formula_implies_trace
+    unfolding weakly_trace_preordered_def
+    by (metis (no_types, lifting) eq_equality in_mono)
 next
   assume \<phi>_eneg: \<open>\<forall>\<phi>\<in>\<O> (E \<infinity> 0 0 0 0 0 0 0). p \<Turnstile>SRBB \<phi> \<longrightarrow> q \<Turnstile>SRBB \<phi>\<close>
   thus \<open>p \<lesssim>WT q\<close>
     unfolding weakly_trace_preordered_def
-    using trace_equals_trace_to_formula trace_formula_to_expressiveness trace_to_srbb_is_trace_formula
+    using trace_equals_trace_to_formula trace_formula_to_expressiveness
+      trace_to_srbb_is_trace_formula
     by fastforce
 qed
 
